LeanColls/Data/List.lean
@@ -7,6 +7,8 @@ import LeanColls.Classes.Seq
 
 import Mathlib.Data.List.Lemmas
 
+open LeanColls
+
 namespace List
 
 @[simp] theorem length_ofFn (f : Fin n → α) : length (ofFn f) = n := by
@@ -29,7 +31,28 @@ namespace List
   : ofFn f = (Array.ofFn f).data := by
   rw [←Array.toList_eq]; rfl
 
-instance : LeanColls.Seq (List τ) τ where
+def snoc? : List α → Option (List α × α)
+| [] => none
+| x::xs =>
+  match snoc? xs with
+  | none => some ([],x)
+  | some (xs',x') => some (x::xs', x')
+
+@[simp] theorem snoc?_eq_none (c : List α) : snoc? c = none ↔ c = [] := by
+  induction c <;> simp_all [snoc?]
+  intro h; split at h <;> simp_all
+
+@[simp] theorem snoc?_eq_some (c : List α) : snoc? c = some (xs,x) ↔ c = xs ++ [x] := by
+  induction c generalizing xs x <;> simp_all [snoc?]
+  case cons hd tl ih =>
+  generalize ho : snoc? tl = o at ih
+  cases o <;> simp_all
+  · cases xs <;> simp
+  · cases xs <;> simp_all
+    · rintro rfl rfl; simp_all; apply ih; rfl
+    · aesop; rw [←ih]; simp
+
+instance : Seq (List τ) τ where
   toList := id
   empty := []
   insert L x := x::L
@@ -38,3 +61,46 @@ instance : LeanColls.Seq (List τ) τ where
   ofFn := List.ofFn
   get := List.get
   set L i x := List.set L i x
+  cons := List.cons
+  cons? := fun | [] => none | x::xs => (x,xs)
+  snoc? := snoc?
+
+
+@[simp] theorem toList_eq (L : List α) : toList L = L := rfl
+
+instance : LawfulSeq (List τ) τ where
+  mem_iff_mem_toList := by simp
+  toList_append := by intros; rfl
+  toMultiset_empty := rfl
+  toMultiset_insert := by intros; rfl
+  toMultiset_singleton := by intro; rfl
+  size_def := by intro; rfl
+  toList_ofFn := by intros; rfl
+  get_def := by intros; rfl
+  toList_set := by intros; rfl
+  cons?_eq_none := by
+    intro c; simp [Seq.cons?]
+    split <;> simp
+  cons?_eq_some := by
+    intro c x c'; simp [Seq.cons?]
+    split <;> simp
+  cons?_eq_some_of_toList := by
+    intro c x c' h; simp_all [Seq.cons?]
+  snoc?_eq_none := by
+    simp [Seq.snoc?]
+  snoc?_eq_some := by
+    simp [Seq.snoc?]
+  snoc?_eq_some_of_toList := by
+    simp [Seq.snoc?]; intros; use ?_
+
+end List
+
+namespace LeanColls.Seq
+
+variable [Seq C τ] [LawfulSeq C τ]
+
+@[simp] theorem size_toList (c : C)
+  : size (toList c) = size c := by
+  simp [size, size_def]
+
+end LeanColls.Seq
